TAO_4_BasicDefinitions.thy
@@ -1,6 +1,6 @@
 (*<*)
-theory TAO_3_BasicDefinitions
-imports TAO_1_Embedding
+theory TAO_4_BasicDefinitions
+imports TAO_3_Quantifiable
 begin
 (*>*)
 
@@ -18,10 +18,13 @@ definition equiv::"\<o>\<Rightarrow>\<o>\<Rightarrow>\<o>" (infixl "\<^bold>\<eq
   "equiv \<equiv> \<lambda> x y . (x \<^bold>\<rightarrow> y) \<^bold>& (y \<^bold>\<rightarrow> x)"
 definition diamond::"\<o>\<Rightarrow>\<o>" ("\<^bold>\<diamond>_" [62] 63) where
   "diamond \<equiv> \<lambda> \<phi> . \<^bold>\<not>\<^bold>\<box>\<^bold>\<not>\<phi>"
+definition (in quantifiable) exists :: "('a\<Rightarrow>\<o>)\<Rightarrow>\<o>" (binder "\<^bold>\<exists>" [8] 9) where
+    "exists \<equiv> \<lambda> \<phi> . \<^bold>\<not>(\<^bold>\<forall> x . \<^bold>\<not>\<phi> x)"
 
 named_theorems conn_defs
 declare diamond_def[conn_defs] conj_def[conn_defs]
         disj_def[conn_defs] equiv_def[conn_defs]
+        exists_def[conn_defs]
 
 subsection{* Abstract and Ordinary Objects *}
 text{* \label{TAO_BasicDefinitions_AbstractOrdinary} *}
@@ -34,29 +37,29 @@ text{* \label{TAO_BasicDefinitions_Identity} *}
 
 definition basic_identity\<^sub>E::"\<Pi>\<^sub>2" where
   "basic_identity\<^sub>E \<equiv> \<^bold>\<lambda>\<^sup>2 (\<lambda> x y . \<lparr>O!,x\<^sup>P\<rparr> \<^bold>& \<lparr>O!,y\<^sup>P\<rparr>
-                         \<^bold>& \<^bold>\<box>(\<^bold>\<forall>\<^sub>1 F. \<lparr>F,x\<^sup>P\<rparr> \<^bold>\<equiv> \<lparr>F,y\<^sup>P\<rparr>))"
+                         \<^bold>& \<^bold>\<box>(\<^bold>\<forall> F. \<lparr>F,x\<^sup>P\<rparr> \<^bold>\<equiv> \<lparr>F,y\<^sup>P\<rparr>))"
 
 definition basic_identity\<^sub>E_infix::"\<kappa>\<Rightarrow>\<kappa>\<Rightarrow>\<o>" (infixl "\<^bold>=\<^sub>E" 63) where
   "x \<^bold>=\<^sub>E y \<equiv> \<lparr>basic_identity\<^sub>E, x, y\<rparr>"
 
 definition basic_identity\<^sub>\<kappa> (infixl "\<^bold>=\<^sub>\<kappa>" 63) where
   "basic_identity\<^sub>\<kappa> \<equiv> \<lambda> x y . (x \<^bold>=\<^sub>E y) \<^bold>\<or> \<lparr>A!,x\<rparr> \<^bold>& \<lparr>A!,y\<rparr>
-                             \<^bold>& \<^bold>\<box>(\<^bold>\<forall>\<^sub>1 F. \<lbrace>x,F\<rbrace> \<^bold>\<equiv> \<lbrace>y,F\<rbrace>)"
+                             \<^bold>& \<^bold>\<box>(\<^bold>\<forall> F. \<lbrace>x,F\<rbrace> \<^bold>\<equiv> \<lbrace>y,F\<rbrace>)"
 
 definition basic_identity\<^sub>1 (infixl "\<^bold>=\<^sub>1" 63) where
-  "basic_identity\<^sub>1 \<equiv> \<lambda> F G . \<^bold>\<box>(\<^bold>\<forall>\<^sub>\<nu> x. \<lbrace>x\<^sup>P,F\<rbrace> \<^bold>\<equiv> \<lbrace>x\<^sup>P,G\<rbrace>)"
+  "basic_identity\<^sub>1 \<equiv> \<lambda> F G . \<^bold>\<box>(\<^bold>\<forall> x. \<lbrace>x\<^sup>P,F\<rbrace> \<^bold>\<equiv> \<lbrace>x\<^sup>P,G\<rbrace>)"
 
 definition basic_identity\<^sub>2 :: "\<Pi>\<^sub>2\<Rightarrow>\<Pi>\<^sub>2\<Rightarrow>\<o>" (infixl "\<^bold>=\<^sub>2" 63) where
-  "basic_identity\<^sub>2 \<equiv> \<lambda> F G .  \<^bold>\<forall>\<^sub>\<nu> x. ((\<^bold>\<lambda>y. \<lparr>F,x\<^sup>P,y\<^sup>P\<rparr>) \<^bold>=\<^sub>1 (\<^bold>\<lambda>y. \<lparr>G,x\<^sup>P,y\<^sup>P\<rparr>))
-                                  \<^bold>& ((\<^bold>\<lambda>y. \<lparr>F,y\<^sup>P,x\<^sup>P\<rparr>) \<^bold>=\<^sub>1 (\<^bold>\<lambda>y. \<lparr>G,y\<^sup>P,x\<^sup>P\<rparr>))"
+  "basic_identity\<^sub>2 \<equiv> \<lambda> F G .  \<^bold>\<forall> x. ((\<^bold>\<lambda>y. \<lparr>F,x\<^sup>P,y\<^sup>P\<rparr>) \<^bold>=\<^sub>1 (\<^bold>\<lambda>y. \<lparr>G,x\<^sup>P,y\<^sup>P\<rparr>))
+                                 \<^bold>& ((\<^bold>\<lambda>y. \<lparr>F,y\<^sup>P,x\<^sup>P\<rparr>) \<^bold>=\<^sub>1 (\<^bold>\<lambda>y. \<lparr>G,y\<^sup>P,x\<^sup>P\<rparr>))"
 
 definition basic_identity\<^sub>3::"\<Pi>\<^sub>3\<Rightarrow>\<Pi>\<^sub>3\<Rightarrow>\<o>" (infixl "\<^bold>=\<^sub>3" 63) where
-  "basic_identity\<^sub>3 \<equiv> \<lambda> F G . \<^bold>\<forall>\<^sub>\<nu> x y. (\<^bold>\<lambda>z. \<lparr>F,z\<^sup>P,x\<^sup>P,y\<^sup>P\<rparr>) \<^bold>=\<^sub>1 (\<^bold>\<lambda>z. \<lparr>G,z\<^sup>P,x\<^sup>P,y\<^sup>P\<rparr>)
-                                   \<^bold>& (\<^bold>\<lambda>z. \<lparr>F,x\<^sup>P,z\<^sup>P,y\<^sup>P\<rparr>) \<^bold>=\<^sub>1 (\<^bold>\<lambda>z. \<lparr>G,x\<^sup>P,z\<^sup>P,y\<^sup>P\<rparr>)
-                                   \<^bold>& (\<^bold>\<lambda>z. \<lparr>F,x\<^sup>P,y\<^sup>P,z\<^sup>P\<rparr>) \<^bold>=\<^sub>1 (\<^bold>\<lambda>z. \<lparr>G,x\<^sup>P,y\<^sup>P,z\<^sup>P\<rparr>)"
+  "basic_identity\<^sub>3 \<equiv> \<lambda> F G . \<^bold>\<forall> x y. (\<^bold>\<lambda>z. \<lparr>F,z\<^sup>P,x\<^sup>P,y\<^sup>P\<rparr>) \<^bold>=\<^sub>1 (\<^bold>\<lambda>z. \<lparr>G,z\<^sup>P,x\<^sup>P,y\<^sup>P\<rparr>)
+                                  \<^bold>& (\<^bold>\<lambda>z. \<lparr>F,x\<^sup>P,z\<^sup>P,y\<^sup>P\<rparr>) \<^bold>=\<^sub>1 (\<^bold>\<lambda>z. \<lparr>G,x\<^sup>P,z\<^sup>P,y\<^sup>P\<rparr>)
+                                  \<^bold>& (\<^bold>\<lambda>z. \<lparr>F,x\<^sup>P,y\<^sup>P,z\<^sup>P\<rparr>) \<^bold>=\<^sub>1 (\<^bold>\<lambda>z. \<lparr>G,x\<^sup>P,y\<^sup>P,z\<^sup>P\<rparr>)"
 
-definition basic_identity\<^sub>\<o>::"\<o>\<Rightarrow>\<o>\<Rightarrow>\<o>" (infixl "\<^bold>=\<^sub>\<o>" 63) where
-  "basic_identity\<^sub>\<o> \<equiv> \<lambda> F G . (\<^bold>\<lambda>y. F) \<^bold>=\<^sub>1 (\<^bold>\<lambda>y. G)"
+definition basic_identity\<^sub>0::"\<o>\<Rightarrow>\<o>\<Rightarrow>\<o>" (infixl "\<^bold>=\<^sub>0" 63) where
+  "basic_identity\<^sub>0 \<equiv> \<lambda> F G . (\<^bold>\<lambda>y. F) \<^bold>=\<^sub>1 (\<^bold>\<lambda>y. G)"
 
 (*<*)
 end
